engine/PrisonersDilemma.lean
@@ -217,4 +217,5 @@ import PrisonersDilemma.Tau.Theorems.TauCupod.Helpers
 import PrisonersDilemma.Tau.Theorems.TauCupod.Phase
 import PrisonersDilemma.Tau.Theorems.TauCIMCIC.Helpers
 import PrisonersDilemma.Tau.Theorems.TauCIMCIC.Phase
+import PrisonersDilemma.Tau.Theorems.TauDIMCID.Helpers
 import PrisonersDilemma.Tau.Theorems.Matrix
